\documentclass[a4paper]{article}
\usepackage[utf8]{inputenc}   % pro unicode UTF-8
\usepackage[czech]{babel} %jazyk dokumentu
\usepackage{listings}
\usepackage{color}
\usepackage[T1]{fontenc}
\usepackage{amssymb}
\usepackage{hyperref}
\usepackage{listingsutf8}
\usepackage{graphicx}
\usepackage{amsmath}
\usepackage{pgfplots}
\usepackage[margin={1cm,2cm}]{geometry}

\graphicspath{ {/} }

\def\doubleunderline#1{\underline{\underline{#1}}}

%%%%%%%%%%%%%%%%%%%%%%%%%%%%%%%%%%%%%%%%%%%%%%%%%%%%%%%%%%%%%

\begin{document}

\noindent
\textbf{Predmet: Mataliza 1}\\
\textbf{Ukol: 9.}\\
\textbf{Verze: 1.}\\
\textbf{Autor: David Napravnik}\\
\textbf{Prezdivka: DN}


\section*{zadani}
$\int \frac{2x}{1-x^2} dx$

\section*{reseni}
pres parcialni zlomky:\\
$\frac{2x}{(1-x)(1+x)}=\frac{A}{1-x}+\frac{B}{1+x}$\\
$2x=A(x+1)+B(1-x)$\\
$A=> x=1 => 2=A(2) => A=1$\\
$B=> x=-1 => -2=B(2) => B=-1$\\
pokracujeme v reseni integralu\\
$\int \frac{1}{1-x} - \int \frac{1}{1+x}~dx$\\
$-\int \frac{1}{x-1} - \int \frac{1}{1+x}~dx$\\
\doubleunderline{$-\log(x-1) - \log(1+x)+c$}\\









\section*{zadani}
$\int \frac{x+1}{x^2+5x+6} dx$

\section*{reseni}
$\int \frac{x+2}{(x+3)(x+2)} - \frac{1}{(x+3)(x+2)}~dx$\\
$\int \frac{1}{(x+3)} - \frac{1}{(x+3)(x+2)}~dx$\\
$\int \frac{1}{(x+3)}~dx - \int \frac{1}{(x+3)(x+2)}~dx$\\
\\
odbocka k parcialnim zlomkum:\\
$\frac{1}{(x+3)(x+2)}=\frac{A}{x+3}+\frac{B}{x+2}$\\
$1=A(x+2)+B(x+3)$\\
$A=-1;~B=1$\\
\\
$\int \frac{1}{(x+3)}~dx - \int\left( \frac{1}{x+2}-\frac{1}{x+3}\right)~dx$\\
$\log(x+3) - (\log(x+2)-\log(x+3)) + c$\\
\doubleunderline{$2*\log(x+3) - \log(x+2) + c$}\\








\section*{zadani}
$\int \frac{x^2-2x-2}{x^2+x-2}~dx$

\section*{reseni}
$\int \frac{x^2+x-2}{x^2+x-2}-\frac{3x}{x^2+x-2}~dx$\\
$\int 1-\frac{3x}{x^2+x-2}~dx$\\
$x - \int \frac{3x}{x^2+x-2}~dx$\\
$x - \int \frac{3x}{(x-1)(x+2)}~dx$\\
odbocka k parcialnim zlomkum:\\
$\frac{3x}{(x-1)(x+2)} = \frac{A}{x-1}+\frac{B}{x+2}$\\
$3x = A(x+2)+B(x-1)$\\
$A=1;~B=2$\\
\\
$x - \int (\frac{1}{x-1} + \frac{2}{x+2})~dx$\\
$x - \int \frac{1}{x-1} - \int \frac{2}{x+2}~dx$\\
\doubleunderline{$x - \log(x-1) - 2\log(x+2)+c$}\\









\section*{zadani}
$\int \frac{3x+5}{x^2+2x+1}~dx$

\section*{reseni}
$\int \frac{1}{x+1} + \frac{2x+4}{(x+1)^2}~dx$\\
$\log(x+1) + 2\int \frac{x+2}{(x+1)^2}~dx$\\
$\log(x+1) + 2\int (\frac{x+1}{(x+1)^2}+\frac{1}{(x+1)^2})~dx$\\
$\log(x+1) + 2\int (\frac{1}{(x+1)}+\frac{1}{(x+1)^2})~dx$\\
$\log(x+1) + 2\int (\frac{1}{(x+1)}) + 2\int(\frac{1}{(x+1)^2})~dx$\\
$\log(x+1) + 2\log(x+1) + 2\int(\frac{1}{(x+1)^2})~dx$\\
$3\log(x+1) + 2\int(\frac{1}{(x+1)^2})~dx$\\
$3\log(x+1) + 2(-\frac{1}{x+1}) + c$\\
\doubleunderline{$3\log(x+1) - \frac{2}{x+1} + c$}\\









\section*{zadani}
$\int x^2 \cos x~dx$

\section*{reseni}
$\int f~dg = fg-\int g~df$\\
\indent $f=x^2;~df=2x$\\
\indent $dg=\cos x;~g=\sin x$\\
$x^2\sin x - 2\int(\sin(x)x)$\\
\indent $f=x;~df=1$\\
\indent $dg=\sin x;~g=-\cos x$\\
$x^2\sin x - 2(-\cos(x)x-\int(-\cos(x)))$\\
$x^2\sin x - 2(-\cos(x)x-(-\sin(x))) + c$\\
\doubleunderline{$x^2\sin x +2\cos(x)x-2\sin(x)$}\\








\section*{zadani}
$\int \frac{1}{(x+1)\sqrt{x}}~dx$

\section*{reseni}
Substituce:\\
$u=\sqrt{x}$\\
\indent$du=\frac{1}{2\sqrt{x}}dx$\\
\indent$dx=2u~du$\\
$\int \frac{1}{(u^2+1)u}~dx$\\
$\int \frac{2u}{(u^2+1)u}~du$\\
$2\int \frac{u}{(u^2+1)u}~du$\\
$2\int \frac{1}{(u^2+1)}~du$\\
$2(\tan^{-1}(u))+c$\\
\doubleunderline{$2(\tan^{-1}(\sqrt{x}))+c$}\\

















\end{document}